src/Narcissus/Examples/NetworkStack/UDP_Packet.v
@@ -19,6 +19,7 @@ Require Import
         Fiat.Narcissus.Common.ComposeIf
         Fiat.Narcissus.Common.ComposeOpt
         Fiat.Narcissus.Formats
+        Fiat.Narcissus.BaseFormats
         Fiat.Narcissus.Stores.EmptyStore
         Fiat.Narcissus.Automation.Solver
         Fiat.Narcissus.Automation.AlignedAutomation.
@@ -26,187 +27,64 @@ Require Import
 Require Import Bedrock.Word.
 
 Import Vectors.VectorDef.VectorNotations.
-Open Scope string_scope.
-Open Scope Tuple_scope.
 
 Section UDP_Decoder.
 
+  Open Scope format_scope.
+
   (* These values are provided by the IP header for checksum calculation.*)
-  Variable srcAddr : word 32.
-  Variable destAddr : word 32.
-  Variable udpLength : word 16.
+  Variable srcAddr : Vector.t (word 8) 4.
+  Variable destAddr : Vector.t (word 8) 4.
+  Variable udpLength : Vector.t (word 8) 2.
 
   Record UDP_Packet :=
     { SourcePort : word 16;
       DestPort : word 16;
       Payload : list (word 8)}.
 
-  Definition UDP_Checksum_Valid
-           (srcAddr : word 32)
-           (destAddr : word 32)
-           (udpLength : word 16)
-           (n : nat)
-           (b : ByteString)
-  := IPChecksum_Valid' (96 + n)
-                (mappend (mappend (AlignedIPChecksum.encode_word srcAddr)
-                (mappend (AlignedIPChecksum.encode_word destAddr)
-                (mappend (AlignedIPChecksum.encode_word (wzero 8))
-                (mappend (AlignedIPChecksum.encode_word (natToWord 8 17))
-                           (AlignedIPChecksum.encode_word udpLength)))))
-                b).
-
   Definition UDP_Packet_Format
-             (udp : UDP_Packet) :=
-         (format_word (udp.(SourcePort))
-    ThenC format_word (udp.(DestPort))
-    ThenC format_nat 16 (8 + |udp.(Payload)|) DoneC)
-    ThenChecksum (UDP_Checksum_Valid srcAddr destAddr udpLength) OfSize 16
-    ThenCarryOn (format_list format_word udp.(Payload) DoneC).
+    : FormatM UDP_Packet ByteString :=
+    (format_word ◦ SourcePort
+     ++ format_word ◦ DestPort
+     ++ format_nat 16 ◦ (Basics.compose (plus 8) (Basics.compose (@length _) Payload)))
+    ThenChecksum (Pseudo_Checksum_Valid srcAddr destAddr udpLength (natToWord 8 17)) OfSize 16
+    ThenCarryOn (format_list format_word ◦ Payload).
 
-
-Definition UDP_encoder_impl (r : UDP_Packet) :=
-( SetCurrentBytes (SourcePort r) >>
-  SetCurrentBytes (DestPort r) >>
-  SetCurrentBytes (natToWord |(Payload r)|) >>
-  SetCurrentBytes (wzero 16) >>
-  AlignedEncodeList (fun c => SetCurrentByte c) (Payload r) >>
-  calculate_Checksum srcAddr destAddr updLength)
   (* The checksum takes three values provided by the IP header for
      checksum calculuation. *)
-
   Definition UDP_Packet_OK (udp : UDP_Packet) :=
     lt (|udp.(Payload)|) (pow2 16 - 8).
 
   (* Step One: Synthesize an encoder and a proof that it is correct. *)
-
-  Arguments NPeano.modulo : simpl never.
-
-  Opaque pow2.
-
   Definition UDP_encoder :
-    CorrectAlignedEncoderFor UDP_Packet_Format UDP_Packet_OK.
+    CorrectAlignedEncoderFor UDP_Packet_Format.
   Proof.
     start_synthesizing_encoder.
-    Print Ltac decompose_aligned_encoder.
-    eapply @CorrectAlignedEncoderForIPChecksumThenC.
-    align_encoder_step.
+    eapply @CorrectAlignedEncoderForPseudoChecksumThenC.
+    Ltac decompose_aligned_encoder :=
+      first [
+          eapply @CorrectAlignedEncoderForIPChecksumThenC
+        | associate_for_ByteAlignment
+        | apply @CorrectAlignedEncoderForThenC
+        | apply @CorrectAlignedEncoderForDoneC].
+    (decompose_aligned_encoder; eauto).
+    (decompose_aligned_encoder; eauto).
+    repeat align_encoder_step.
+    eapply CorrectAlignedEncoderForFormat2Nat.
+    simpl; eauto.
+    simpl; eauto.
+    repeat align_encoder_step.
+    repeat align_encoder_step.
+    repeat align_encoder_step.
   Defined.
 
   (* Step Two: Extract the encoder function, and have it start encoding
      at the start of the provided ByteString [v]. *)
   Definition UDP_encoder_impl r {sz} v :=
-    Eval simpl in (projT1 UDP_encoder r sz v 0 tt).
+    Eval simpl in (projT1 UDP_encoder sz v 0 r tt).
 
 (* Step Two and a Half: Add some simple facts about correct packets
    for the decoder automation. *)
-Lemma UDP_Packet_Header_Len_eq
-  : forall packet len,
-    UDP_Packet_Header_Len packet = len
-    -> ((|packet.(Options) |) = len - 5).
-Proof.
-  unfold UDP_Packet_Header_Len; intros.
-  apply Minus.plus_minus.
-  rewrite H; reflexivity.
-Qed.
-
-Lemma UDP_Packet_Header_Len_bound
-  : forall packet,
-    UDP_Packet_OK packet ->
-    lt (UDP_Packet_Header_Len packet) (pow2 4)%nat.
-Proof.
-  intros; replace (pow2 4) with 16 by reflexivity.
-  unfold UDP_Packet_OK in H; unfold UDP_Packet_Header_Len.
-  omega.
-Qed.
-
-Hint Resolve UDP_Packet_Header_Len_eq : data_inv_hints.
-Hint Resolve UDP_Packet_Header_Len_bound : data_inv_hints.
-
-(* Step Three: Synthesize a decoder and a proof that /it/ is correct. *)
-Definition UDP_Packet_Header_decoder
-  : CorrectAlignedDecoderFor UDP_Packet_OK UDP_Packet_Format.
-Proof.
-  (* We have to use an extra lemma at the start, because of the 'exotic'
-     IP Checksum. *)
-  eapply CorrectAlignedDecoderForIPChecksumThenC.
-  repeat calculate_length_ByteString.
-  (* Once that's done, the normal automation works just fine :) *)
-  synthesize_aligned_decoder.
-Defined.
-
-(* Step Four: Extract the decoder function, and have /it/ start decoding
-   at the start of the provided ByteString [v]. *)
-Arguments GetCurrentBytes : simpl never.
-Definition UDP_decoder_impl {sz} v :=
-  Eval simpl in (projT1 UDP_Packet_Header_decoder sz v 0 ()).
-
-
-
-
-
-(*Lemma refine_IfDec_Under_Bind {B} P (P_dec : Decidable P)
-  : forall (tb eb : Comp B) tb' eb',
-    (forall (p : P), refine tb (tb' p))
-    -> (forall (np : ~ P), refine eb (eb' np))
-    -> refine (IfDec P Then tb Else eb)
-              (match Decidable_witness as b return Decidable_witness = b -> _ with
-               | true => fun H => tb' (Decidable_sound P _ H)
-               | false => fun H => eb' (Decidable_complete_alt P _ H)
-               end eq_refl).
-Proof.
-  unfold IfDec_Then_Else; intros.
-  computes_to_econstructor.
-  eapply PickComputes; apply Decidable_witness_decides.
-  revert v H1;
-    generalize (Decidable_sound P P_dec) (Decidable_complete_alt P P_dec).
-  destruct Decidable_witness; intros; eauto.
-  eapply H; eauto.
-  eapply H0; eauto.
-Qed. *)
-
-
-Import Vectors.VectorDef.VectorNotations.
-Open Scope string_scope.
-Open Scope Tuple_scope.
-
-(* Start Example Derivation. *)
-
-Section UDP_Decoder.
-
-  (* These values are provided by the IP header for checksum calculation.*)
-  Variable srcAddr : word 32.
-  Variable destAddr : word 32.
-  Variable udpLength : word 16.
-
-Definition UDP_Packet :=
-  @Tuple <"SourcePort" :: word 16,
-          "DestPort" :: word 16,
-          "Payload" :: list char >.
-
-Definition UDP_Checksum_Valid
-           (srcAddr : word 32)
-           (destAddr : word 32)
-           (udpLength : word 16)
-           (n : nat)
-           (b : ByteString)
-  := IPChecksum_Valid (96 + n)
-                (mappend (mappend (IPChecksum.encode_word srcAddr)
-                (mappend (IPChecksum.encode_word destAddr)
-                (mappend (IPChecksum.encode_word (wzero 8))
-                (mappend (IPChecksum.encode_word (natToWord 8 17))
-                           (IPChecksum.encode_word udpLength)))))
-                b).
-
-Definition format_UDP_Packet_Spec
-           (udp : UDP_Packet) :=
-          (format_word (udp!"SourcePort")
-    ThenC format_word (udp!"DestPort")
-    ThenC format_nat 16 (8 + |udp!"Payload"|) DoneC)
-    ThenChecksum (UDP_Checksum_Valid srcAddr destAddr udpLength) OfSize 16
-    ThenCarryOn (format_list format_word udp!"Payload" DoneC).
-
-Definition UDP_Packet_OK (udp : UDP_Packet) :=
-lt (|udp!"Payload"|) (pow2 16 - 8).
 
 Definition UDP_Packet_formatd_measure (udp_b : ByteString)
   : nat :=
@@ -217,20 +95,16 @@ Definition UDP_Packet_formatd_measure (udp_b : ByteString)
   | None => 0
   end.
 
-Arguments NPeano.modulo : simpl never.
-
-Opaque pow2.
-
-Lemma UDP_Packet_Header_Len_OK
+(*Lemma UDP_Packet_Header_Len_OK
   : forall (a : UDP_Packet) (ctx ctx' ctx'' : CacheFormat) (c : word 16) (b b'' ext : ByteString),
-    (format_word (a!"SourcePort")
-                      ThenC format_word (a!"DestPort")
-                      ThenC format_nat 16 (8 + |a!"Payload"|) DoneC) ctx ↝
+    (format_word (a.(SourcePort))
+                      ThenC format_word (a.(DestPort))
+                      ThenC format_nat 16 (8 + |a.(Payload)|) DoneC) ctx ↝
                                                                             (b, ctx') ->
-    (format_list format_word a!"Payload" DoneC) ctx' ↝ (b'', ctx'') ->
-    (lt (|a!"Payload"|) (pow2 16 - 8))%nat ->
+    (format_list format_word a.(Payload) DoneC) ctx' ↝ (b'', ctx'') ->
+    (lt (|a.(Payload)|) (pow2 16 - 8))%nat ->
     (fun _ : UDP_Packet => 16 + (16 + (16 + length_ByteString ByteString_id))) a +
-    (fun a0 : UDP_Packet => (|a0!"Payload" |) * 8 + length_ByteString ByteString_id) a + 16 =
+    (fun a0 : UDP_Packet => (|a0.(Payload) |) * 8 + length_ByteString ByteString_id) a + 16 =
     UDP_Packet_formatd_measure
       (mappend (mappend b (mappend (format_checksum ByteString monoid ByteString_QueueMonoidOpt 16 c) b'')) ext).
 Proof.
@@ -260,37 +134,66 @@ Proof.
   rewrite <- Compare_dec.nat_compare_lt.
   rewrite Npow2_nat.
   omega.
-Qed.
+Qed. *)
 
-Definition UDP_Packet_decoder
-  : CorrectDecoderFor UDP_Packet_OK format_UDP_Packet_Spec.
+Lemma UDP_Packet_Header_Len_bound
+  : forall data : UDP_Packet,
+    UDP_Packet_OK data ->
+    lt (8 + (| Payload data |)) (pow2 16).
 Proof.
+Admitted.
+
+Opaque pow2.
+
+Hint Resolve UDP_Packet_Header_Len_bound : data_inv_hints.
+Arguments GetCurrentBytes : simpl never.
+(* Step Three: Synthesize a decoder and a proof that /it/ is correct. *)
+Definition UDP_Packet_Header_decoder
+  : CorrectAlignedDecoderFor UDP_Packet_OK UDP_Packet_Format.
+Proof.
+  (* We have to use an extra lemma at the start, because of the 'exotic'
+     IP Checksum. *)
+  eapply CorrectAlignedDecoderForUDPChecksumThenC.
+  repeat calculate_length_ByteString.
+  (* Once that's done, the normal automation works just fine :) *)
   start_synthesizing_decoder.
-  normalize_compose monoid.
-  apply_IPChecksum_dep UDP_Packet_Header_Len_OK.
-
-  unfold UDP_Packet_OK; clear; intros ? H'; simpl; intuition eauto using lt_minus_plus.
-  eapply lt_minus_plus with (m := 8); eauto.
-
-  decode_step idtac.
-  decode_step idtac.
-  decode_step idtac.
-  simpl; intros; intuition.
-  decompose_pair_hyp.
-  instantiate (1 := fst (snd (snd proj)) - 8);
-    rewrite <- H4.
-  auto with arith.
-  decode_step idtac.
-  decode_step idtac.
-
+  match goal with
+  | |- CorrectDecoder ?monoid _ _ _ _ _ => normalize_compose monoid
+  end.
+  decode_step ltac:(idtac).
+  decode_step ltac:(idtac).
+  decode_step ltac:(idtac).
+  decode_step ltac:(idtac).
+  decode_step ltac:(idtac).
+  decode_step ltac:(idtac).
+  decode_step ltac:(idtac).
+  decode_step ltac:(idtac).
+  decode_step ltac:(idtac).
+  decode_step ltac:(idtac).
+  decode_step ltac:(idtac).
+  decode_step ltac:(idtac).
+  decode_step ltac:(idtac).
+  decode_step ltac:(idtac).
+  decode_step ltac:(idtac).
+  decode_step ltac:(idtac).
+  simpl; intros; intuition; instantiate (1 := proj1 -8); omega.
+  decode_step ltac:(idtac).
+  decode_step ltac:(idtac).
+  cbv beta; synthesize_cache_invariant.
+  (* Perform algebraic simplification of the decoder implementation. *)
+  cbv beta; unfold decode_nat; optimize_decoder_impl.
+  cbv beta; align_decoders.
+  Grab Existential Variables.
+  shelve.
   synthesize_cache_invariant.
-  repeat optimize_decoder_impl.
-
 Defined.
 
-Definition UDP_Packet_decoder_impl :=
-  Eval simpl in (fst (proj1_sig UDP_Packet_decoder)).
+(* Step Four: Extract the decoder function, and have /it/ start decoding
+   at the start of the provided ByteString [v]. *)
+
+Definition UDP_decoder_impl {sz} v :=
+  Eval simpl in (projT1 UDP_Packet_Header_decoder sz v 0 ()).
 
 End UDP_Decoder.
 
-Print UDP_Packet_decoder_impl.
+Print UDP_decoder_impl.
