src/Narcissus/Formats/Base/SequenceFormat.v
@@ -2,6 +2,7 @@ Require Import
         Fiat.Computation
         Fiat.Common.DecideableEnsembles
         Fiat.Narcissus.Common.Specs
+        Fiat.Narcissus.Common.ComposeOpt
         Fiat.Narcissus.Common.Notations
         Fiat.Narcissus.Formats.Base.FMapFormat
         Fiat.Narcissus.Formats.Base.LaxTerminalFormat.
@@ -15,10 +16,7 @@ Section SequenceFormat.
   Definition sequence_Format
              {S : Type}
              (format1 format2 : FormatM S T)
-    := (fun s env =>
-          `(t1, env') <- format1 s env ;
-          `(t2, env'') <- format2 s env';
-           ret (mappend t1 t2, env''))%comp.
+    := (fun s => compose _ (format1 s) (format2 s))%comp.
 
   Definition sequence_Decode
              {S S' : Type}
@@ -61,7 +59,7 @@ Section SequenceFormat.
     : CorrectEncoder (format1 ++ format2)
                      (sequence_Encode encode1 encode2).
   Proof.
-    unfold CorrectEncoder, sequence_Encode, sequence_Format,
+    unfold CorrectEncoder, sequence_Encode, sequence_Format, compose,
     DecodeBindOpt, BindOpt in *; intuition; intros.
     - destruct (encode1 a env) as [ [t1 xxenv] | ] eqn: ? ;
         simpl in *; try discriminate.
@@ -102,7 +100,7 @@ Section SequenceFormat.
                            (sequence_Decode decode1 decode2).
   Proof.
     unfold CorrectDecoder_simpl, Projection_Format,
-    sequence_Decode, sequence_Format, FMap_Format; split; intros.
+    sequence_Decode, sequence_Format, compose, Compose_Format; split; intros.
     - unfold Bind2 in H0; computes_to_inv; subst.
       eapply format1_overlap in H0; destruct_ex; split_and.
       rewrite @unfold_computes in H0'.
@@ -113,7 +111,7 @@ Section SequenceFormat.
         eauto.
       rewrite decode1_eq; eauto.
       eapply H3; eauto.
-      unfold Restrict_Format, FMap_Format; apply unfold_computes.
+      unfold Restrict_Format, Compose_Format; apply unfold_computes.
       setoid_rewrite unfold_computes; eexists; intuition eauto.
     - destruct (decode1 bin env') as [ [ [s' t'] xenv'']  | ] eqn: ?; try discriminate.
       destruct decode1_correct as [decode1_correct' decode1_correct].
@@ -124,7 +122,7 @@ Section SequenceFormat.
       eapply decode2_correct in H0; eauto.
       destruct_ex; split_and.
       eexists; intuition eauto.
-      unfold Restrict_Format, FMap_Format, LaxTerminal_Format, sequence_Format,
+      unfold Restrict_Format, Compose_Format, LaxTerminal_Format, sequence_Format,
         Bind2 in *; computes_to_inv.
       rewrite @unfold_computes in H1.
       destruct_ex; split_and; simpl in *; subst.
@@ -138,14 +136,14 @@ Section SequenceFormat.
         (format2 : FormatM S T)
         (decode1 : DecodeM (S' * T) T)
         (decode2 : S' -> DecodeM S T)
-        (decode1_correct : CorrectDecoder_simpl (Projection_Format fst format1 ++ ?* ) decode1)
+        (decode1_correct : CorrectDecoder_simpl (Projection_Format format1 fst ++ ?* ) decode1)
         (decode2_correct : forall (s' : S'), CorrectDecoder_simpl (Restrict_Format (fun s => f s = s') format2) (decode2 s'))
-    : CorrectDecoder_simpl (Projection_Format f format1 ++ format2)
+    : CorrectDecoder_simpl (Projection_Format format1 f ++ format2)
                            (sequence_Decode decode1 decode2).
   Proof.
     unfold Projection_Format.
     eapply (CorrectDecoder_sequence (fun s s' => f s = s')); eauto; intros;
-      unfold Projection_Format, FMap_Format, sequence_Format, Bind2, LaxTerminal_Format in *.
+      unfold Projection_Format, Compose_Format, sequence_Format, compose, Bind2, LaxTerminal_Format in *.
     - rewrite @unfold_computes in H.
       destruct_ex; split_and; subst.
       eexists; intros; intuition.
@@ -157,6 +155,69 @@ Section SequenceFormat.
       eexists; simpl; intuition eauto.
       destruct v; apply unfold_computes; eauto.
   Qed.
+
+  (*Corollary CorrectDecoder_sequence_Done
+            {S : Type}
+            (P : S -> Prop)
+            (format : FormatM (S * T) T)
+            (s : S)
+            (singleton_format : forall (s' : S) (t : T) env tenv',
+                format (s', t) env ∋ tenv' <-> s' = s
+                                               /\ fst tenv' = mempty
+                                               /\ snd tenv' = env)
+    : CorrectDecoder_simpl (format ++ ?* ) (LaxTerminal_Decode s).
+  Proof.
+    unfold CorrectDecoder_simpl, LaxTerminal_Format,
+    LaxTerminal_Decode, sequence_Format, Compose_Format; split; intros.
+    - unfold Bind2 in H0; computes_to_inv; subst.
+      injections.
+      destruct data; eapply singleton_format in H0; simpl in *; intuition; subst.
+      destruct v; simpl in *; subst.
+      eexists; split; eauto.
+      rewrite mempty_left; reflexivity.
+    - injections; unfold Bind2; eexists.
+
+      simpl.
+      destruct v; destruct v0; simpl in *; injections.
+      destruct decode1_correct as [? _].
+      destruct (decode2_correct x) as [? _].
+      destruct (H0 env env' c (x, t0) (mappend t t0)) as (xenv', (decode1_eq, Equiv_xenv));
+        eauto.
+      rewrite decode1_eq; eauto.
+      eapply H3; eauto.
+      unfold Restrict_Format, Compose_Format; apply unfold_computes.
+      setoid_rewrite unfold_computes; eexists; intuition eauto.
+    - destruct (decode1 bin env') as [ [ [s' t'] xenv'']  | ] eqn: ?; try discriminate.
+      destruct decode1_correct as [decode1_correct' decode1_correct].
+      specialize (decode2_correct s'); destruct decode2_correct as [_ decode2_correct].
+      generalize Heqo; intro Heqo'.
+      eapply decode1_correct in Heqo; eauto.
+      destruct_ex; split_and.
+      eapply decode2_correct in H0; eauto.
+      destruct_ex; split_and.
+      eexists; intuition eauto.
+      unfold Restrict_Format, Compose_Format, LaxTerminal_Format, sequence_Format,
+        Bind2 in *; computes_to_inv.
+      rewrite @unfold_computes in H1.
+      destruct_ex; split_and; simpl in *; subst.
+      eapply format1'_overlap in H2; destruct_ex; split_and; subst; eauto.
+  Qed.
+    unfold
+
+    eapply (CorrectDecoder_sequence (fun s s' => f s = s')); eauto; intros;
+      unfold Projection_Format, Compose_Format, sequence_Format, Bind2, LaxTerminal_Format in *.
+    - rewrite @unfold_computes in H.
+      destruct_ex; split_and; subst.
+      eexists; intros; intuition.
+      destruct tenv'; simpl; computes_to_econstructor.
+      rewrite unfold_computes; eauto.
+      simpl; computes_to_econstructor; eauto.
+    - computes_to_inv; subst.
+      apply_in_hyp @unfold_computes; destruct_ex; split_and; subst.
+      eexists; simpl; intuition eauto.
+      destruct v; apply unfold_computes; eauto.
+  Qed. *)
+
 
 End SequenceFormat.
 
