src/Narcissus/Automation/AlignedAutomation.v
@@ -6,6 +6,7 @@ Require Import
         Fiat.Narcissus.Common.ComposeCheckSum
         Fiat.Narcissus.Common.ComposeIf
         Fiat.Narcissus.Formats
+        Fiat.Narcissus.BaseFormats
         Fiat.Narcissus.Automation.Solver.
 
 Require Import Bedrock.Word.
@@ -27,14 +28,14 @@ Ltac align_decoders_step :=
     | eapply @AlignedDecodeBindCharM; intros; eauto
     | eapply @AlignedDecodeBind4CharM; intros; eauto
     | eapply @AlignedDecodeBindEnumM; intros; eauto
-    | eapply @AlignedDecodeBindUnused2CharM; simpl;
+    | eapply @AlignedDecodeBindUnused2CharM; simpl; eauto;
       eapply DecodeMEquivAlignedDecodeM_trans;
       [ | intros; reflexivity
         |  ]
-    |   eapply @AlignedDecodeBindUnusedCharM; simpl;
-        eapply DecodeMEquivAlignedDecodeM_trans;
-        [ | intros; reflexivity
-          | intros ]
+    | eapply @AlignedDecodeBindUnusedCharM; simpl; eauto;
+      eapply DecodeMEquivAlignedDecodeM_trans;
+      [ | intros; reflexivity
+        |  ]
     | eapply @AlignedDecodeListM; intros; eauto
     | eapply @AlignedDecodeCharM; intros; eauto
     | eapply (fun H H' => @AlignedDecodeNCharM _ _ H H' 4); eauto; simpl; intros
@@ -44,9 +45,10 @@ Ltac align_decoders_step :=
     | eapply @AlignedDecode_Sumb
     | eapply @AlignedDecode_ifb
     | intros; higher_order_reflexivity
-    |   eapply AlignedDecode_CollapseWord';
+    |   eapply @AlignedDecode_CollapseWord';
         eauto using decode_word_eq_decode_unused_word,
         decode_word_eq_decode_bool,
+        decode_word_eq_decode_nat,
         decode_word_eq_decode_word
     ].
 
@@ -92,12 +94,13 @@ Proof.
   unfold ByteString_id, length_ByteString; simpl; omega.
 Qed.
 
-Lemma length_ByteString_unused_word
-  : forall (sz : nat) (b : ByteString) (ctx ctx' : CacheFormat),
-    format_unused_word sz ctx ↝ (b, ctx') -> length_ByteString b = sz.
+Lemma length_ByteString_unused_word {S}
+  : forall (s : S) (sz : nat) (b : ByteString) (ctx ctx' : CacheFormat),
+    format_unused_word sz s ctx ↝ (b, ctx') -> length_ByteString b = sz.
 Proof.
-  unfold format_unused_word, format_unused_word';
-    intros; computes_to_inv; injections.
+  unfold format_unused_word, Compose_Format;
+    intros; rewrite unfold_computes in H; destruct_ex; split_and.
+  unfold format_word in H0; computes_to_inv; injections.
   rewrite length_encode_word'; simpl.
   unfold ByteString_id, length_ByteString; simpl; omega.
 Qed.
@@ -106,7 +109,7 @@ Lemma length_ByteString_bool
   : forall (b : bool) (bs : ByteString) (ctx ctx' : CacheFormat),
     format_bool b ctx ↝ (bs, ctx') -> length_ByteString bs = 1.
 Proof.
-  unfold format_bool, format_unused_word';
+  unfold format_bool;
     intros; computes_to_inv; injections.
   reflexivity.
 Qed.
@@ -135,21 +138,79 @@ Proof.
   erewrite length_ByteString_enqueue_ByteString, H0, H1; eauto with arith.
 Qed.
 
+
 Ltac eapply_in_hyp lem :=
   match goal with
   | H:_ |- _ => eapply lem in H; [ | clear H | .. | clear H]
   end.
 
+Lemma length_ByteString_map {S S'}
+  : forall (sz : nat) (f : S -> S') (format : FormatM S' _) (s : S) (b : ByteString) (ctx ctx' : CacheFormat),
+    (format (f s) ctx ∋ (b, ctx') -> length_ByteString b = sz)
+    -> Projection_Format format f s ctx ∋ (b, ctx') -> length_ByteString b = sz.
+Proof.
+  unfold Projection_Format, Compose_Format; intros.
+  rewrite unfold_computes in H0; destruct_ex; intuition; subst.
+  eapply H; eauto.
+Qed.
+
+Corollary length_ByteString_map_word {S}
+  : forall (sz : nat) (f : S -> word sz) (s : S) (b : ByteString) (ctx ctx' : CacheFormat),
+    Projection_Format format_word f s ctx ∋ (b, ctx') -> length_ByteString b = sz.
+Proof.
+  intros; eapply length_ByteString_map; eauto using length_ByteString_word.
+Qed.
+
+Corollary length_ByteString_map_nat {S}
+  : forall (sz : nat) (f : S -> nat) (s : S) (b : ByteString) (ctx ctx' : CacheFormat),
+    Projection_Format (format_nat sz) f s ctx ∋ (b, ctx') -> length_ByteString b = sz.
+Proof.
+  unfold format_nat; intros.
+  apply EquivFormat_Projection_Format in H.
+  eauto using length_ByteString_word.
+Qed.
+
+Corollary length_ByteString_map_bool {S}
+  : forall (f : S -> bool) (s : S) (b : ByteString) (ctx ctx' : CacheFormat),
+    Projection_Format format_bool f s ctx ∋ (b, ctx') -> length_ByteString b = 1.
+Proof.
+  intros; eapply length_ByteString_map; eauto using length_ByteString_bool.
+Qed.
+
+Corollary length_ByteString_map_enum {S'}
+  : forall (len sz : nat)
+           (codes : Vector.t (word sz) (S len))
+           (f : S' -> Fin.t (S len)) (s : S') (b : ByteString) (ctx ctx' : CacheFormat),
+    Projection_Format (format_enum codes) f s ctx ∋ (b, ctx') -> length_ByteString b = sz.
+Proof.
+  intros; eapply length_ByteString_map; eauto.
+  eauto using length_ByteString_word.
+Qed.
+
 Ltac associate_for_ByteAlignment :=
   eapply @Guarded_CorrectAlignedEncoderThenCAssoc;
-  [clear; intros ce bs ce' Comp;
-   repeat first [ apply_in_hyp length_ByteString_word
-                | apply_in_hyp length_ByteString_unused_word
-                | apply_in_hyp length_ByteString_bool
-                | eapply_in_hyp length_ByteString_compose;
+  [clear; intros ce bs ce' Comp ? ;
+   repeat first [ apply_in_hyp @length_ByteString_map_word
+                | apply_in_hyp @length_ByteString_map_bool
+                | apply_in_hyp @length_ByteString_word
+                | apply_in_hyp @length_ByteString_unused_word
+                | apply_in_hyp @length_ByteString_bool
+                | apply_in_hyp @length_ByteString_map_nat
+                | apply_in_hyp @length_ByteString_map_enum
+                | eapply_in_hyp @length_ByteString_compose;
                   [ | clear; intros | .. | clear; intros ]
                 | eassumption]; omega
   | ].
+
+(*Lemma CorrectAlignedEncoderForFormatOption {S}
+     : forall (format_Some : FormatM S ByteString) (encode_A : forall sz : nat, AlignedEncodeM sz),
+       CorrectAlignedEncoder format_A encode_A ->
+       CorrectAlignedEncoder (format_list format_A) (AlignedEncodeList encode_A)
+
+Lemma
+  CorrectAlignedEncoder
+    (Option.format_option format_word (format_unused_word 16) ◦ UrgentPointer ++
+     format_list format_word ◦ Options ++ format_list format_word ◦ Payload) ?encode_A *)
 
 (*Lemma CollapseCorrectAlignedEncoderFormatWord
       (addE_addE_plus :
@@ -172,12 +233,14 @@ Proof.
   repeat computes_to_econstructor; eauto.
 Qed. *)
 
-Lemma refine_format_unused_word
-  : forall sz ce,
-    refine (format_unused_word sz ce) (format_word (wzero sz) ce).
+Lemma refine_format_unused_word {S}
+  : forall sz (s : S) ce,
+    refine (format_unused_word sz s ce) (format_word (wzero sz) ce).
 Proof.
-  intros; unfold format_unused_word, format_unused_word'.
-  repeat computes_to_econstructor; eauto.
+  intros; unfold format_unused_word, Compose_Format;
+    intros ? ?.
+  apply unfold_computes; eexists; split; eauto.
+  apply unfold_computes; eauto.
 Qed.
 
 Lemma refine_format_bool
@@ -188,7 +251,67 @@ Proof.
   reflexivity.
 Qed.
 
-Ltac calculate_length_ByteString :=
+Lemma refine_format_bool_map {S}
+      (f : S -> bool)
+  : forall s ce,
+    refine (FMapFormat.Projection_Format format_bool f s ce) (FMapFormat.Projection_Format format_word (fun s => (WS (f s) WO)) s ce).
+Proof.
+  intros; unfold FMapFormat.Projection_Format, FMapFormat.Compose_Format; intros ? ?.
+  rewrite unfold_computes in H; destruct_ex; intuition.
+  apply unfold_computes; eexists; split; eauto; subst.
+  eapply refine_format_bool; eauto.
+Qed.
+
+Lemma refine_format_nat_map {S}
+      {sz}
+      (f : S -> nat)
+  : forall s ce,
+    refine (FMapFormat.Projection_Format (format_nat sz) f s ce)
+           (FMapFormat.Projection_Format format_word (Basics.compose (natToWord sz) f) s ce).
+Proof.
+  intros; unfold FMapFormat.Projection_Format, FMapFormat.Compose_Format, format_nat; intros ? ?.
+  rewrite unfold_computes in H; destruct_ex; intuition.
+  apply unfold_computes; eexists; split; eauto; subst.
+  eauto.
+Qed.
+
+Lemma refine_format_unused_word_map {S}
+  : forall sz (s : S) ce,
+    refine (format_unused_word sz s ce) (FMapFormat.Projection_Format format_word (fun s => wzero sz) s ce).
+Proof.
+  unfold format_unused_word, FMapFormat.Projection_Format, Compose_Format; intros;
+    intros ? ?.
+  rewrite unfold_computes in H; destruct_ex; intuition; subst.
+  apply unfold_computes; eexists; split; eauto.
+  apply unfold_computes; eauto.
+Qed.
+
+Lemma refine_format_word_map {S}
+      {sz}
+      (f : S -> word sz)
+  : forall s ce,
+    refine (FMapFormat.Projection_Format format_word f s ce) (format_word (f s) ce).
+Proof.
+  intros; unfold FMapFormat.Projection_Format, FMapFormat.Compose_Format; intros ? ?.
+  apply unfold_computes; eexists; split; eauto.
+Qed.
+
+  Lemma length_ByteString_Projection {S S'}:
+    forall (format1 : FormatM S ByteString)
+           (f : S' -> S)
+           (b : ByteString) s (ctx ctx' : CacheFormat)
+           (n : nat),
+      (Projection_Format format1 f)%format s ctx ↝ (b, ctx') ->
+      (forall (ctx0 : CacheFormat) (b0 : ByteString) (ctx'0 : CacheFormat),
+          format1 (f s) ctx0 ↝ (b0, ctx'0) -> length_ByteString b0 = n) ->
+      length_ByteString b = n.
+  Proof.
+    intros.
+    eapply H0.
+    eapply EquivFormat_Projection_Format; eauto.
+  Qed.
+
+  Ltac calculate_length_ByteString :=
   intros;
   match goal with
   | H:_ ↝ _
@@ -200,8 +323,9 @@ Ltac calculate_length_ByteString :=
          try (simpl mempty; rewrite length_ByteString_ByteString_id)
        | eapply (length_ByteString_compose _ _ _ _ _ _ _ H);
          try (simpl mempty; rewrite length_ByteString_ByteString_id)
+       | eapply (length_ByteString_Projection _ _ _ _ _ _ _ H)
        | eapply (fun H' H'' => length_ByteString_format_option _ _ _ _ _ _ _ H' H'' H)
-       | eapply (length_ByteString_unused_word _ _ _ _ H)
+       | eapply (length_ByteString_unused_word _ _ _ _ _ H)
        | eapply (length_ByteString_bool _ _ _ _ H)
        | eapply (length_ByteString_word _ _ _ _ _ H)
        | eapply (fun H' => length_ByteString_format_list _ _ _ _ _ _ H' H)
@@ -209,37 +333,39 @@ Ltac calculate_length_ByteString :=
     clear H
   end.
 
-
 Ltac collapse_unaligned_words :=
   intros; eapply refine_CorrectAlignedEncoder;
-  [ eauto ; intros; try set_refine_evar; repeat eapply refine_CollapseFormatWord; intros;
-    unfold format_nat; eauto using refine_format_bool, refine_format_unused_word;
-    reflexivity
+  [repeat (eauto ; intros; eapply refine_CollapseFormatWord'; eauto);
+   unfold format_nat; eauto using refine_format_bool, refine_format_unused_word_map,
+                      refine_format_bool_map, refine_format_unused_word,
+                      refine_format_nat_map;
+   reflexivity
   | ].
-
-Ltac decompose_aligned_encoder :=
-  repeat first [
-           eapply @CorrectAlignedEncoderForIPChecksumThenC
-         | associate_for_ByteAlignment
-         | match goal with
-             |- context[ByteString_id] => apply @CorrectAlignedEncoderForThenC
-           end
-         | apply @CorrectAlignedEncoderForDoneC].
 
 Ltac start_synthesizing_encoder :=
   lazymatch goal with
-  | |- CorrectAlignedEncoderFor ?Invariant ?Spec =>
-    try unfold Spec; try unfold Invariant
+  | |- CorrectAlignedEncoderFor ?Spec =>
+    try unfold Spec
   end;
   (* Memoize any string constants *)
   (*pose_string_hyps; *)
   eexists; simpl; intros.
 
+Ltac decompose_aligned_encoder :=
+  first [
+           eapply @CorrectAlignedEncoderForIPChecksumThenC
+         | first [ associate_for_ByteAlignment
+                 | apply @CorrectAlignedEncoderForThenC]
+         | apply @CorrectAlignedEncoderForDoneC].
+
 Ltac align_encoder_step :=
   first
-    [ (*apply CorrectAlignedEncoderForFormatList*) fail
+    [ apply CorrectAlignedEncoderForFormatList
     | apply CorrectAlignedEncoderForFormatChar; eauto
     | apply CorrectAlignedEncoderForFormatNat
+    | apply CorrectAlignedEncoderForFormatEnum
+    | eapply CorrectAlignedEncoderProjection
+    | eapply CorrectAlignedEncoderForFormatUnusedWord
     | intros; eapply CorrectAlignedEncoderForFormatNChar with (sz := 2); eauto
     | intros; eapply CorrectAlignedEncoderForFormatNChar with (sz := 3); eauto
     | intros; eapply CorrectAlignedEncoderForFormatNChar with (sz := 4); eauto
@@ -251,5 +377,5 @@ Ltac align_encoder :=
 
 Ltac synthesize_aligned_encoder :=
   start_synthesizing_encoder;
-  decompose_aligned_encoder;
+  decompose_aligned_encoder; eauto;
   repeat align_encoder_step.
